C-verifier/src/Midend-IVL/Isabelle-UTP-Extended/HoareLogic/PartialCorrectness/utp_hoare.thy
@@ -20,191 +20,892 @@ theory utp_hoare
 imports "../../utp/utp_rec_total"
 begin
 
-named_theorems hoare and hoare_safe
+named_theorems hoare_sp_rules and hoare_wp_rules and hoare_wp_proof_annotation_rules
 
-method hoare_split uses hr = 
-  ((simp add: assigns_r_comp usubst unrest)?, -- {* Eliminate assignments where possible *}
-   (auto 
-    intro: hoare intro!: hoare_safe hr
-    simp add: assigns_r_comp conj_comm conj_assoc usubst unrest))[1] -- {* Apply Hoare logic laws *}
-
-method hoare_auto uses hr = (hoare_split hr: hr; rel_auto?)
-  
 subsection {*Hoare triple definition*}
 
-text {*A Hoare triple is represented by a pre-condition @{text P} a post-condition @{text Q}
-       and a program @{text C}. It says whenever the pre-condition @{text P} holds on the initial state
-       then the post-condition @{text Q} must hold on the final state and this 
-       after the execution of the program @{text C}.*}
 
 definition hoare_r :: "'\<alpha> cond \<Rightarrow> '\<alpha> hrel \<Rightarrow> '\<alpha> cond \<Rightarrow> bool" ("\<lbrace>_\<rbrace>_\<lbrace>_\<rbrace>\<^sub>u") where
 "\<lbrace>p\<rbrace>Q\<lbrace>r\<rbrace>\<^sub>u = ((\<lceil>p\<rceil>\<^sub>< \<Rightarrow> \<lceil>r\<rceil>\<^sub>>) \<sqsubseteq> Q)"
 
-declare hoare_r_def [upred_defs]
+declare hoare_r_def[upred_defs]
+lemma hoare_true_assisgns_prog_t: 
+  "\<lbrace>p\<rbrace> \<langle>\<sigma>\<rangle>\<^sub>a \<lbrace>true\<rbrace>\<^sub>u"
+  by rel_simp
 
-lemma hoare_true [hoare]: "\<lbrace>p\<rbrace>C\<lbrace>true\<rbrace>\<^sub>u"
-  by rel_auto
+lemma skip_true_hoare_rel: 
+  "\<lbrace>p\<rbrace>SKIP\<^sub>r\<lbrace>true\<rbrace>\<^sub>u"
+   by rel_simp
 
-lemma hoare_false [hoare]: "\<lbrace>false\<rbrace>C\<lbrace>q\<rbrace>\<^sub>u"
-  by rel_auto
+lemma pre_false_hoare_rel: 
+  "\<lbrace>false\<rbrace>C\<lbrace>q\<rbrace>\<^sub>u"
+  by rel_simp
 
-subsection {*Hoare for Consequence*}
+subsection {*Precondition weakening*}
 
-lemma hoare_r_conseq [hoare]: 
-  assumes "`p\<^sub>1 \<Rightarrow> p\<^sub>2`" and "\<lbrace>p\<^sub>2\<rbrace>C\<lbrace>q\<^sub>2\<rbrace>\<^sub>u" and "`q\<^sub>2 \<Rightarrow> q\<^sub>1`" 
-  shows   "\<lbrace>p\<^sub>1\<rbrace>C\<lbrace>q\<^sub>1\<rbrace>\<^sub>u"
-  by (insert assms) rel_auto
-
-subsection {*Precondition strengthening*}
-
-lemma hoare_pre_str[hoare]:
+lemma pre_str_hoare_rel:
   assumes "`p\<^sub>1 \<Rightarrow> p\<^sub>2`" and "\<lbrace>p\<^sub>2\<rbrace>C\<lbrace>q\<rbrace>\<^sub>u"
   shows "\<lbrace>p\<^sub>1\<rbrace>C\<lbrace>q\<rbrace>\<^sub>u" 
-  by (insert assms) rel_auto
-
-subsection {*Post-condition weakening*}
-
-lemma hoare_post_weak[hoare]:
+  using assms  
+  by rel_simp
+    
+subsection {*Post-condition strengthening*}
+  
+lemma post_weak_hoare_rel:
   assumes "\<lbrace>p\<rbrace>C\<lbrace>q\<^sub>2\<rbrace>\<^sub>u" and "`q\<^sub>2 \<Rightarrow> q\<^sub>1`"
   shows "\<lbrace>p\<rbrace>C\<lbrace>q\<^sub>1\<rbrace>\<^sub>u" 
- by (insert assms) rel_auto
-
+  using assms  
+  by rel_simp
+    
+subsection {*Consequence rule*}  
+  
+lemma consequence_hoare_rel:
+  assumes I0': "`p \<Rightarrow> p'`" 
+  assumes induct_step:"\<lbrace>p'\<rbrace> C \<lbrace>q'\<rbrace>\<^sub>u" 
+  assumes I0 :"`q'\<Rightarrow> q`"  
+  shows "\<lbrace>p\<rbrace>C\<lbrace>q\<rbrace>\<^sub>u"
+proof(rule post_weak_hoare_rel[OF _ I0], goal_cases)
+  case 1
+  then show ?case by (rule pre_str_hoare_rel[OF I0' induct_step]) 
+qed   
+  
 subsection {*Hoare and assertion logic*}
 
-lemma hoare_r_conj [hoare]: 
-  assumes"\<lbrace>p\<rbrace>C\<lbrace>r\<rbrace>\<^sub>u" and "\<lbrace>p\<rbrace>C\<lbrace>s\<rbrace>\<^sub>u"  
+lemma conj_hoare_rel: 
+  assumes"\<lbrace>p\<rbrace>C\<lbrace>r\<rbrace>\<^sub>u" and "\<lbrace>p\<rbrace>C\<lbrace>s\<rbrace>\<^sub>u"
   shows "\<lbrace>p\<rbrace>C\<lbrace>r \<and> s\<rbrace>\<^sub>u"
-  by (insert assms) rel_auto
-
+  using assms  
+  by rel_simp
+    
 subsection {*Hoare SKIP*}
 
-lemma skip_hoare_r [hoare_safe]: "\<lbrace>p\<rbrace>II\<lbrace>p\<rbrace>\<^sub>u"
-  by rel_auto
-
+lemma skip_rel_hoare_rel[hoare_sp_rules, hoare_wp_rules, hoare_wp_proof_annotation_rules]: 
+  "\<lbrace>p\<rbrace>SKIP\<^sub>r\<lbrace>p\<rbrace>\<^sub>u"
+  by rel_simp
+    
+lemma skip_rel_hoare_rel_intro: 
+  "`p \<Rightarrow> q`\<Longrightarrow>\<lbrace>p\<rbrace>SKIP\<^sub>r\<lbrace>q\<rbrace>\<^sub>u"
+  by rel_simp
+  
 subsection {*Hoare for assignment*}
 
-lemma assigns_hoare_r [hoare_safe]:
-  assumes"`p \<Rightarrow> \<sigma> \<dagger> q`"
+lemma assigns_rel_hoare_rel_intro: 
+  assumes"`p \<Rightarrow> \<sigma> \<dagger> q`" 
   shows  "\<lbrace>p\<rbrace>\<langle>\<sigma>\<rangle>\<^sub>a\<lbrace>q\<rbrace>\<^sub>u"
-  by (insert assms) rel_auto
-
-lemma assigns_hoare_r' [hoare]: "\<lbrace>\<sigma> \<dagger> p\<rbrace>\<langle>\<sigma>\<rangle>\<^sub>a\<lbrace>p\<rbrace>\<^sub>u"
-  by rel_auto
-
-lemma assigns_naive_rule:
-  assumes "x\<sharp>e" and "weak_lens x" 
-  shows   "\<lbrace>p\<rbrace>x :== e\<lbrace>&x=\<^sub>ue\<rbrace>\<^sub>u"
-  using assms
-  by pred_simp   
+  using assms  
+  by rel_simp
     
-lemma assigns_floyd_r [hoare]:
-  assumes \<open>vwb_lens x\<close>
-  shows   \<open>\<lbrace>p\<rbrace>x :== e\<lbrace>\<^bold>\<exists>v \<bullet> p\<lbrakk>\<guillemotleft>v\<guillemotright>/x\<rbrakk> \<and> &x =\<^sub>u e\<lbrakk>\<guillemotleft>v\<guillemotright>/x\<rbrakk>\<rbrace>\<^sub>u\<close>
-  apply (insert assms)
-  apply pred_simp
-  apply transfer
-  apply (rule_tac x = \<open>get\<^bsub>x\<^esub> a\<close> in exI)
-  (*subgoal for a x p e
-   apply (rule exI[where x="get\<^bsub>x\<^esub> a"])*)
-  apply auto
-  done
+lemma assigns_rel_backward_hoare_rel[hoare_wp_rules, hoare_wp_proof_annotation_rules]: 
+  "\<lbrace>\<sigma> \<dagger> p\<rbrace>\<langle>\<sigma>\<rangle>\<^sub>a\<lbrace>p\<rbrace>\<^sub>u"
+  by rel_simp
+    
+lemma assigns_rel_floyd_hoare_rel[hoare_sp_rules]:
+  assumes "vwb_lens x"
+  shows \<open>\<lbrace>p\<rbrace>x :== e\<lbrace>\<^bold>\<exists>v \<bullet> p\<lbrakk>\<guillemotleft>v\<guillemotright>/x\<rbrakk> \<and> &x =\<^sub>u e\<lbrakk>\<guillemotleft>v\<guillemotright>/x\<rbrakk>\<rbrace>\<^sub>u\<close>
+  using assms
+  apply rel_simp   
+  subgoal for a    
+    apply (rule exI[where x = "lens_get x a"])
+    apply simp
+    done
+  done    
 
 subsection {*Hoare for Sequential Composition*}
 
-lemma seq_hoare_r:
-  assumes"\<lbrace>p\<rbrace>C\<^sub>1\<lbrace>s\<rbrace>\<^sub>u" and "\<lbrace>s\<rbrace>C\<^sub>2\<lbrace>r\<rbrace>\<^sub>u"
-  shows"\<lbrace>p\<rbrace>C\<^sub>1 ;; C\<^sub>2\<lbrace>r\<rbrace>\<^sub>u"
-  by (insert assms) rel_auto
+lemma seq_invariant_hoare_rel: 
+ "\<lbrakk>\<lbrace>p\<rbrace>Q\<^sub>1\<lbrace>p\<rbrace>\<^sub>u ; \<lbrace>p\<rbrace>Q\<^sub>2\<lbrace>p\<rbrace>\<^sub>u\<rbrakk> \<Longrightarrow> \<lbrace>p\<rbrace>Q\<^sub>1 ;; Q\<^sub>2\<lbrace>p\<rbrace>\<^sub>u"
+  by rel_simp 
     
-lemma seq_hoare_invariant [hoare_safe]: 
-  assumes "\<lbrace>p\<rbrace>Q\<^sub>1\<lbrace>p\<rbrace>\<^sub>u" and "\<lbrace>p\<rbrace>Q\<^sub>2\<lbrace>p\<rbrace>\<^sub>u" 
-  shows "\<lbrace>p\<rbrace>Q\<^sub>1 ;; Q\<^sub>2\<lbrace>p\<rbrace>\<^sub>u"
-  using assms 
-  by (auto simp: seq_hoare_r)
+lemma seq_stronger_pre_1_hoare_rel: 
+  "\<lbrakk> \<lbrace>p \<and> q\<rbrace>Q\<^sub>1\<lbrace>p \<and> q\<rbrace>\<^sub>u ; \<lbrace>p \<and> q\<rbrace>Q\<^sub>2\<lbrace>q\<rbrace>\<^sub>u \<rbrakk> \<Longrightarrow> \<lbrace>p \<and> q\<rbrace>Q\<^sub>1 ;; Q\<^sub>2\<lbrace>q\<rbrace>\<^sub>u"
+  by rel_simp
 
-lemma seq_hoare_stronger_pre_1 [hoare_safe]: 
-  assumes "\<lbrace>p \<and> q\<rbrace>Q\<^sub>1\<lbrace>p \<and> q\<rbrace>\<^sub>u" and "\<lbrace>p \<and> q\<rbrace>Q\<^sub>2\<lbrace>q\<rbrace>\<^sub>u" 
-  shows "\<lbrace>p \<and> q\<rbrace>Q\<^sub>1 ;; Q\<^sub>2\<lbrace>q\<rbrace>\<^sub>u"
-  using assms 
-  by (auto simp: seq_hoare_r)
-
-lemma seq_hoare_stronger_pre_2 [hoare_safe]: 
-  assumes "\<lbrace>p \<and> q\<rbrace>Q\<^sub>1\<lbrace>p \<and> q\<rbrace>\<^sub>u" and "\<lbrace>p \<and> q\<rbrace>Q\<^sub>2\<lbrace>p\<rbrace>\<^sub>u" 
-  shows "\<lbrace>p \<and> q\<rbrace>Q\<^sub>1 ;; Q\<^sub>2\<lbrace>p\<rbrace>\<^sub>u"
-  using assms 
-  by (auto simp: seq_hoare_r)
-   
-lemma seq_hoare_inv_r_2 [hoare]: 
-  assumes "\<lbrace>p\<rbrace>Q\<^sub>1\<lbrace>q\<rbrace>\<^sub>u" and "\<lbrace>q\<rbrace>Q\<^sub>2\<lbrace>q\<rbrace>\<^sub>u" 
-  shows   "\<lbrace>p\<rbrace>Q\<^sub>1 ;; Q\<^sub>2\<lbrace>q\<rbrace>\<^sub>u"
-  using assms 
-  by (auto simp: seq_hoare_r)
- 
-lemma seq_hoare_inv_r_3 [hoare]: 
-  assumes "\<lbrace>p\<rbrace>Q\<^sub>1\<lbrace>p\<rbrace>\<^sub>u" and "\<lbrace>p\<rbrace>Q\<^sub>2\<lbrace>q\<rbrace>\<^sub>u" 
-  shows "\<lbrace>p\<rbrace>Q\<^sub>1 ;; Q\<^sub>2\<lbrace>q\<rbrace>\<^sub>u"
-  using assms 
-  by (auto simp: seq_hoare_r)
+lemma seq_stronger_pre_2_hoare_rel: 
+  "\<lbrakk> \<lbrace>p \<and> q\<rbrace>Q\<^sub>1\<lbrace>p \<and> q\<rbrace>\<^sub>u ; \<lbrace>p \<and> q\<rbrace>Q\<^sub>2\<lbrace>p\<rbrace>\<^sub>u\<rbrakk> \<Longrightarrow> \<lbrace>p \<and> q\<rbrace>Q\<^sub>1 ;; Q\<^sub>2\<lbrace>p\<rbrace>\<^sub>u"
+  by rel_simp
+    
+lemma seq_hoare_rel[hoare_wp_rules, hoare_sp_rules]: 
+  assumes"\<lbrace>p\<rbrace>C\<^sub>1\<lbrace>s\<rbrace>\<^sub>u" and "\<lbrace>s\<rbrace>C\<^sub>2\<lbrace>r\<rbrace>\<^sub>u" 
+  shows"\<lbrace>p\<rbrace>C\<^sub>1 ;; C\<^sub>2\<lbrace>r\<rbrace>\<^sub>u"
+  using assms
+  by rel_simp
     
 subsection {*Hoare for Conditional*}
 
-lemma cond_hoare_r [hoare_safe]: 
+lemma cond_rel_hoare_rel: 
   assumes "\<lbrace>b \<and> p\<rbrace>C\<^sub>1\<lbrace>q\<rbrace>\<^sub>u" and "\<lbrace>\<not>b \<and> p\<rbrace>C\<^sub>2\<lbrace>q\<rbrace>\<^sub>u" 
-  shows "\<lbrace>p\<rbrace>C\<^sub>1 \<triangleleft> b \<triangleright>\<^sub>r C\<^sub>2\<lbrace>q\<rbrace>\<^sub>u"
-  by (insert assms) rel_auto
-
-subsection {*Hoare for assert*}
-
-lemma assert_hoare_r [hoare_safe]: 
-  assumes "\<lbrace>c \<and> p\<rbrace>II\<lbrace>q\<rbrace>\<^sub>u" and "\<lbrace>\<not>c \<and> p\<rbrace>true\<lbrace>q\<rbrace>\<^sub>u" 
-  shows "\<lbrace>p\<rbrace>c\<^sub>\<bottom>\<lbrace>q\<rbrace>\<^sub>u"
-  unfolding rassert_def using assms cond_hoare_r [of c p _ q ]
-  by auto
-
-subsection {*Hoare for assume*}
-
-lemma assume_hoare_r [hoare_safe]: 
-  assumes "\<lbrace>c \<and> p\<rbrace>II\<lbrace>q\<rbrace>\<^sub>u" and "\<lbrace>\<not>c \<and> p\<rbrace>false\<lbrace>q\<rbrace>\<^sub>u" 
-  shows "\<lbrace>p\<rbrace>c\<^sup>\<top>\<lbrace>q\<rbrace>\<^sub>u"
-  unfolding rassume_def using assms cond_hoare_r [of c p _ q ]
-  by auto
-
-subsection {*Hoare for While-loop*}
-
-lemma while_hoare_r [hoare_safe]:
-  assumes "\<lbrace>p \<and> b\<rbrace>C\<lbrace>p\<rbrace>\<^sub>u"
-  shows "\<lbrace>p\<rbrace>while b do C od\<lbrace>\<not>b \<and> p\<rbrace>\<^sub>u"
+  shows "\<lbrace>p\<rbrace> bif b then C\<^sub>1 else C\<^sub>2 eif\<lbrace>q\<rbrace>\<^sub>u"
   using assms
-  apply (simp add: while_def hoare_r_def)
-  apply (rule_tac lfp_lowerbound) 
-  apply(rel_auto)
-  done
-
-lemma while_hoare_r' [hoare_safe]:
-  assumes "\<lbrace>p \<and> b\<rbrace>C\<lbrace>p\<rbrace>\<^sub>u" and "`p \<and> \<not>b \<Rightarrow> q`"
-  shows "\<lbrace>p\<rbrace>while b do C od\<lbrace>q\<rbrace>\<^sub>u"
-  using assms
-  by (metis conj_comm hoare_r_conseq p_imp_p taut_true while_hoare_r)
-
-lemma while_invr_hoare_r  [hoare_safe]:
-  assumes "\<lbrace>p \<and> b\<rbrace>C\<lbrace>p\<rbrace>\<^sub>u" and "`pre \<Rightarrow> p`" and "`(\<not>b \<and> p) \<Rightarrow> post`"
-  shows "\<lbrace>pre\<rbrace>while b invr p do C od\<lbrace>post\<rbrace>\<^sub>u"
-  by (metis assms hoare_r_conseq while_hoare_r while_inv_def)
-
-text {* Frame rule: If starting $S$ in a state satisfying $p establishes q$ in the final state, then
-  we can insert an invariant predicate $r$ when $S$ is framed by $a$, provided that $r$ does not
-  refer to variables in the frame, and $q$ does not refer to variables outside the frame. *}
+  by pred_simp
     
-lemma frame_hoare_r [hoare_safe]: 
-  assumes "vwb_lens a" "a \<sharp> r" "a \<natural> q" "\<lbrace>p \<and> r\<rbrace>S\<lbrace>q\<rbrace>\<^sub>u"
-  shows "\<lbrace>p \<and> r\<rbrace>a:[S]\<lbrace>q \<and> r\<rbrace>\<^sub>u"
-  using assms by (rel_simp)
-
-lemma frame_hoare_r' [hoare_safe]: 
-  assumes "vwb_lens a" "a \<sharp> r" "a \<natural> q" "\<lbrace>r \<and> p\<rbrace>S\<lbrace>q\<rbrace>\<^sub>u"
-  shows "\<lbrace>r \<and> p\<rbrace>a:[S]\<lbrace>r \<and> q\<rbrace>\<^sub>u"
+lemma cond_rel_hoare_rel_wp[hoare_wp_rules, hoare_wp_proof_annotation_rules]: 
+  assumes "\<lbrace>p'\<rbrace>C\<^sub>1\<lbrace>q\<rbrace>\<^sub>u" and "\<lbrace>p''\<rbrace>C\<^sub>2\<lbrace>q\<rbrace>\<^sub>u"
+  shows "\<lbrace>(b \<and> p')\<or> (\<not>b \<and> p'')\<rbrace>bif b then C\<^sub>1 else C\<^sub>2 eif\<lbrace>q\<rbrace>\<^sub>u"
   using assms
-  by (simp add: frame_hoare_r utp_pred_laws.inf.commute)    
+  by pred_simp
+    
+lemma cond_rel_hoare_rel_sp[hoare_sp_rules]:
+  assumes \<open>\<lbrace>b \<and> p\<rbrace>C\<^sub>1\<lbrace>q\<rbrace>\<^sub>u\<close> and \<open>\<lbrace>\<not>b \<and> p\<rbrace>C\<^sub>2\<lbrace>s\<rbrace>\<^sub>u\<close>
+  shows \<open>\<lbrace>p\<rbrace>bif b then C\<^sub>1 else C\<^sub>2 eif\<lbrace>q \<or> s\<rbrace>\<^sub>u\<close>
+  using assms
+  by pred_simp
+    
+subsection {*Hoare for recursion*}
+  
+lemma nu_rel_hoare_rel_partial: 
+  assumes induct_step:
+    "\<And> st P. \<lbrace>p\<rbrace>P\<lbrace>q\<rbrace>\<^sub>u \<Longrightarrow> \<lbrace>p\<rbrace>F P\<lbrace>q\<rbrace>\<^sub>u"   
+  shows "\<lbrace>p\<rbrace>\<nu> F \<lbrace>q\<rbrace>\<^sub>u"  
+  unfolding hoare_r_def
+  apply (rule lfp_lowerbound)
+    apply (rule induct_step[unfolded hoare_r_def])
+    apply simp
+  done    
+  
+lemma mu_rel_hoare_rel:
+  assumes WF: "wf R"
+  assumes M:"mono F"  
+  assumes induct_step:
+    "\<And> st P. \<lbrace>p \<and>(e,\<guillemotleft>st\<guillemotright>)\<^sub>u\<in>\<^sub>u\<guillemotleft>R\<guillemotright>\<rbrace>P\<lbrace>q\<rbrace>\<^sub>u \<Longrightarrow> \<lbrace>p \<and> e =\<^sub>u \<guillemotleft>st\<guillemotright>\<rbrace>F P\<lbrace>q\<rbrace>\<^sub>u"   
+  shows "\<lbrace>p\<rbrace>\<mu> F \<lbrace>q\<rbrace>\<^sub>u"  
+  unfolding hoare_r_def
+proof (rule mu_rec_total_utp_rule[OF WF M , of _ e ], goal_cases)
+  case (1 st)
+  then show ?case 
+  by (rule induct_step[unfolded hoare_r_def], simp)    
+qed
+    
+lemma mu_rel_hoare_rel':
+  assumes WF: "wf R"
+  assumes M:"mono F"  
+  assumes induct_step:
+    "\<And> st P. \<lbrace>p \<and>(e,\<guillemotleft>st\<guillemotright>)\<^sub>u\<in>\<^sub>u\<guillemotleft>R\<guillemotright>\<rbrace> P \<lbrace>q\<rbrace>\<^sub>u \<Longrightarrow> \<lbrace>p \<and> e =\<^sub>u \<guillemotleft>st\<guillemotright>\<rbrace> F P \<lbrace>q\<rbrace>\<^sub>u" 
+  assumes I0: "`p' \<Rightarrow> p`"  
+  shows "\<lbrace>p'\<rbrace>\<mu> F \<lbrace>q\<rbrace>\<^sub>u"
+  by (simp add: pre_str_hoare_rel[OF I0 mu_rel_hoare_rel[OF WF M induct_step]])
+
+subsection {*Hoare for frames*}
+  
+lemma antiframe_hoare_rel:
+  assumes "vwb_lens a"
+  assumes "a \<sharp> r" 
+  assumes "a \<natural> q"    
+  assumes "\<lbrace>p\<rbrace>P\<lbrace>q\<rbrace>\<^sub>u"  
+  shows "\<lbrace>p \<and> r\<rbrace>a:[P]\<lbrace>q \<and> r\<rbrace>\<^sub>u"
+  using assms
+  by rel_simp  
+  
+lemma antiframe_hoar_rel_stronger:
+  assumes "vwb_lens a"
+  assumes "a \<sharp> r" 
+  assumes "a \<natural> q"    
+  assumes "\<lbrace>p \<and> r\<rbrace>P\<lbrace>q\<rbrace>\<^sub>u"  
+  shows "\<lbrace>p \<and> r\<rbrace>a:[P]\<lbrace>q \<and> r\<rbrace>\<^sub>u"
+  using assms
+  by rel_simp
+    
+lemma frame_hoare_rel:
+  assumes "vwb_lens a"
+  assumes "a \<natural> r" 
+  assumes "a \<sharp> q"    
+  assumes "\<lbrace>p\<rbrace>P\<lbrace>q\<rbrace>\<^sub>u"  
+  shows "\<lbrace>p \<and> r\<rbrace> a:\<lbrakk>P\<rbrakk> \<lbrace>q \<and> r\<rbrace>\<^sub>u"
+  using assms
+  by rel_simp
+    
+lemma frame_hoare_rel_stronger:
+  assumes "vwb_lens a"
+  assumes "a \<natural> r" 
+  assumes "a \<sharp> q"    
+  assumes "\<lbrace>p \<and> r\<rbrace>P\<lbrace>q\<rbrace>\<^sub>u"  
+  shows "\<lbrace>p \<and> r\<rbrace> a:\<lbrakk>P\<rbrakk> \<lbrace>q \<and> r\<rbrace>\<^sub>u"
+  using assms 
+  by rel_simp
+    
+lemma blah1: 
+  assumes "vwb_lens g'" "vwb_lens l"
+  assumes  "l \<bowtie> g'" 
+  shows "vwb_lens  (g' +\<^sub>L l)" 
+  using assms 
+  by (simp add: lens_indep_sym plus_vwb_lens) 
+   
+lemma
+  assumes 1:"vwb_lens g" 
+  assumes 2:"vwb_lens g'" 
+  assumes 3:"vwb_lens l"
+  assumes 4:"l \<bowtie> g" 
+  assumes 8:"g' \<subseteq>\<^sub>L g"
+  assumes 5:"{&g', &l}:[C] = C" 
+  assumes 6:"\<lbrace>p\<rbrace>C\<lbrace>q\<rbrace>\<^sub>u"
+  assumes 7:"`r \<Rightarrow> p`"     
+  shows "\<lbrace>r\<rbrace> l:\<lbrakk>C\<rbrakk> \<lbrace>(\<exists> l \<bullet> q) \<and> (\<exists>g' \<bullet> r)\<rbrace>\<^sub>u"
+  using 1 2 3 4 5 6 7 unfolding lens_indep_def
+  apply rel_auto 
+   apply (metis (no_types, lifting) vwb_lens_wb wb_lens.get_put)
+  apply (rule_tac x="get\<^bsub> g'\<^esub> a" in exI) using 8 4
+proof -
+  fix a :: 'b and x :: 'b
+  assume a1: "\<lbrakk>r\<rbrakk>\<^sub>e a"
+  assume a2: "\<forall>\<sigma> v u. put\<^bsub>l\<^esub> (put\<^bsub>g\<^esub> \<sigma> v) u = put\<^bsub>g\<^esub> (put\<^bsub>l\<^esub> \<sigma> u) v"
+  assume a3: "vwb_lens g"
+  assume a4: "\<lbrakk>C\<rbrakk>\<^sub>e (a, x)"
+  assume a5: "\<forall>a b. (\<exists>x. \<lbrakk>C\<rbrakk>\<^sub>e (a, x) \<and> b = put\<^bsub>g'\<^esub> (put\<^bsub>l\<^esub> a (get\<^bsub>l\<^esub> x)) (get\<^bsub>g'\<^esub> x)) = \<lbrakk>C\<rbrakk>\<^sub>e (a, b)"
+  assume a6: "vwb_lens l"
+  assume a7: "\<forall>\<sigma> u. get\<^bsub>g\<^esub> (put\<^bsub>l\<^esub> \<sigma> u) = get\<^bsub>g\<^esub> \<sigma>"
+  assume a8: "vwb_lens g'"
+  have f9: "\<forall>l la b c a. \<not> mwb_lens l \<or> \<not> la \<subseteq>\<^sub>L l \<or> put\<^bsub>l\<^esub> (put\<^bsub>la\<^esub> (b::'b) (c::'c)) (a::'a) = put\<^bsub>l\<^esub> b a"
+    by (meson sublens_put_put)
+  have "mwb_lens g"
+    using a3 vwb_lens_mwb by blast
+  then have f10: "put\<^bsub>g\<^esub> (put\<^bsub>g'\<^esub> (put\<^bsub>l\<^esub> a (get\<^bsub>l\<^esub> (v2_0 x a))) (get\<^bsub>g'\<^esub> (v2_0 x a))) (get\<^bsub>g\<^esub> x) = put\<^bsub>g\<^esub> (put\<^bsub>l\<^esub> a (get\<^bsub>l\<^esub> (v2_0 x a))) (get\<^bsub>g\<^esub> x)"
+    using f9 by (metis "8") (* > 1.0 s, timed out *)
+  obtain bb :: "'b \<Rightarrow> 'b \<Rightarrow> 'b" where
+    "\<forall>x0 x1. (\<exists>v2. \<lbrakk>C\<rbrakk>\<^sub>e (x1, v2) \<and> x0 = put\<^bsub>g'\<^esub> (put\<^bsub>l\<^esub> x1 (get\<^bsub>l\<^esub> v2)) (get\<^bsub>g'\<^esub> v2)) = (\<lbrakk>C\<rbrakk>\<^sub>e (x1, bb x0 x1) \<and> x0 = put\<^bsub>g'\<^esub> (put\<^bsub>l\<^esub> x1 (get\<^bsub>l\<^esub> (bb x0 x1))) (get\<^bsub>g'\<^esub> (bb x0 x1)))"
+    by moura
+  then have f11: "\<lbrakk>C\<rbrakk>\<^sub>e (a, bb x a) \<and> x = put\<^bsub>g'\<^esub> (put\<^bsub>l\<^esub> a (get\<^bsub>l\<^esub> (bb x a))) (get\<^bsub>g'\<^esub> (bb x a))"
+    using a5 a4 by presburger
+  have "mwb_lens g"
+    using a3 vwb_lens_mwb by blast
+  then have f12: "put\<^bsub>g\<^esub> (put\<^bsub>g'\<^esub> a (get\<^bsub>g'\<^esub> (bb x a))) (get\<^bsub>g\<^esub> x) = put\<^bsub>g\<^esub> a (get\<^bsub>g\<^esub> x)"
+    using f9 by (metis "8")
+  have f13: "\<forall>l la b c. \<not> vwb_lens l \<or> \<not> la \<subseteq>\<^sub>L l \<or> get\<^bsub>l\<^esub> (put\<^bsub>la\<^esub> (b::'b) (c::'c)) = put\<^bsub>la /\<^sub>L l\<^esub> (get\<^bsub>l\<^esub> b::'a) c"
+    by (simp add: lens_get_put_quasi_commute)
+  then have f14: "get\<^bsub>g\<^esub> (put\<^bsub>g'\<^esub> a (get\<^bsub>g'\<^esub> (bb x a))) = put\<^bsub>g' /\<^sub>L g\<^esub> (get\<^bsub>g\<^esub> a) (get\<^bsub>g'\<^esub> (bb x a))"
+    using a3 "8" by fastforce 
+  have "get\<^bsub>g\<^esub> (put\<^bsub>g'\<^esub> (put\<^bsub>l\<^esub> a (get\<^bsub>l\<^esub> (bb x a))) (get\<^bsub>g'\<^esub> (bb x a))) = put\<^bsub>g' /\<^sub>L g\<^esub> (get\<^bsub>g\<^esub> (put\<^bsub>l\<^esub> a (get\<^bsub>l\<^esub> (bb x a)))) (get\<^bsub>g'\<^esub> (bb x a))"
+    using a3 f13 "8" by fastforce 
+  then show "\<lbrakk>r\<rbrakk>\<^sub>e (put\<^bsub>g'\<^esub> (put\<^bsub>l\<^esub> x (get\<^bsub>l\<^esub> a)) (get\<^bsub>g'\<^esub> a))"
+    using f14 f12 f11 f10 a8 a7 a6 a3 a2 a1
+  proof -
+    have "\<forall>l la b c a. \<not> mwb_lens l \<or> \<not> la \<subseteq>\<^sub>L l \<or> put\<^bsub>l\<^esub> (put\<^bsub>la\<^esub> (b::'b) (c::'c)) (a::'a) = put\<^bsub>l\<^esub> b a"
+      by (meson sublens_put_put)
+    then have "put\<^bsub>g\<^esub> (put\<^bsub>g'\<^esub> (put\<^bsub>l\<^esub> a (get\<^bsub>l\<^esub> (bb x a))) (get\<^bsub>g'\<^esub> (bb x a))) (put\<^bsub>g' /\<^sub>L g\<^esub> (get\<^bsub>g\<^esub> (put\<^bsub>l\<^esub> a (get\<^bsub>l\<^esub> (bb x a)))) (get\<^bsub>g'\<^esub> (bb x a))) = put\<^bsub>g\<^esub> (put\<^bsub>l\<^esub> a (get\<^bsub>l\<^esub> (bb x a))) (put\<^bsub>g' /\<^sub>L g\<^esub> (get\<^bsub>g\<^esub> (put\<^bsub>l\<^esub> a (get\<^bsub>l\<^esub> (bb x a)))) (get\<^bsub>g'\<^esub> (bb x a)))"
+      by (metis "8" \<open>mwb_lens g\<close>) 
+    then show ?thesis
+      by (metis (no_types) \<open>get\<^bsub>g\<^esub> (put\<^bsub>g'\<^esub> (put\<^bsub>l\<^esub> a (get\<^bsub>l\<^esub> (bb x a))) (get\<^bsub>g'\<^esub> (bb x a))) = put\<^bsub>g' /\<^sub>L g\<^esub> (get\<^bsub>g\<^esub> (put\<^bsub>l\<^esub> a (get\<^bsub>l\<^esub> (bb x a)))) (get\<^bsub>g'\<^esub> (bb x a))\<close> a1 a2 a3 a6 a7 a8 f11 f12 f14 vwb_lens.put_eq vwb_lens_wb wb_lens.get_put)
+  qed
+qed
+
+subsection {*Hoare for while loop*} 
+  
+lemma if_rel_mono:
+  "mono (\<lambda>X. bif b then P ;; X else Q eif)"
+  by (auto intro: monoI seqr_mono cond_mono) 
+
+
+lemma while_gfp_hoare_rel_minimal_partial:
+  assumes seq_step: "`p \<Rightarrow> invar`"
+  assumes induct_step: "\<lbrace>invar\<and> b\<rbrace> C \<lbrace>invar\<rbrace>\<^sub>u"  
+  shows "\<lbrace>p\<rbrace>while\<^sup>\<top> b do C od\<lbrace>\<not>b \<and> invar\<rbrace>\<^sub>u"
+  unfolding while_gfp_rel_def_alt
+  apply (rule pre_str_hoare_rel[OF seq_step])   
+  apply (rule nu_rel_hoare_rel_partial)
+  apply (rule cond_rel_hoare_rel)  
+   apply (rule seq_hoare_rel[where s="invar"])
+  subgoal for st P
+    using pre_str_hoare_rel induct_step seq_step
+    unfolding hoare_r_def
+    apply pred_simp
+    done
+  subgoal for st P
+    apply assumption
+    done
+  subgoal for st P
+    apply pred_simp
+    done
+  done          
+
+lemma while_gfp_invr_hoare_rel_minimal_partial:
+  assumes seq_step: "`p \<Rightarrow> invar`"
+  assumes induct_step: "\<lbrace>invar\<and> b\<rbrace> C \<lbrace>invar\<rbrace>\<^sub>u"  
+  shows "\<lbrace>p\<rbrace>invr invar while\<^sup>\<top> b do C od\<lbrace>\<not>b \<and> invar\<rbrace>\<^sub>u"
+  unfolding while_gfp_invr_rel_def 
+  by (auto intro!: assms while_gfp_hoare_rel_minimal_partial)
+    
+lemma while_gfp_rel_consequence_partial:
+  assumes seq_step: "`p\<Rightarrow>invar`"
+  assumes PHI: "`\<not>b \<and> invar \<Rightarrow> q`"
+  assumes I0': "` invar \<and> b  \<Rightarrow> p'`"
+  assumes induct_step: "\<lbrace>p'\<rbrace>C \<lbrace>q'\<rbrace>\<^sub>u"
+  assumes I0: "`q' \<Rightarrow> invar`"  
+  shows "\<lbrace>p\<rbrace>while\<^sup>\<top> b do C od\<lbrace>q\<rbrace>\<^sub>u"
+  by (rule consequence_hoare_rel[OF seq_step _ PHI, 
+                                 OF while_gfp_hoare_rel_minimal_partial[OF uimp_refl],
+                                 OF consequence_hoare_rel[OF I0' induct_step I0]])
+
+lemma while_gfp_invr_rel_consequence_partial:
+  assumes seq_step: "`p\<Rightarrow>invar`"
+  assumes PHI: "`\<not>b \<and> invar \<Rightarrow> q`"
+  assumes I0': "` invar \<and> b  \<Rightarrow> p'`"
+  assumes induct_step: "\<lbrace>p'\<rbrace>C \<lbrace>q'\<rbrace>\<^sub>u"
+  assumes I0: "`q' \<Rightarrow> invar`"  
+  shows "\<lbrace>p\<rbrace>invr invar while\<^sup>\<top> b do C od\<lbrace>q\<rbrace>\<^sub>u"
+  unfolding while_gfp_invr_rel_def 
+  by (auto intro!: assms while_gfp_rel_consequence_partial)  
+
+lemma while_gfp_rel_wp_partial:
+  assumes PHI: "`\<not>b \<and> invar \<Rightarrow> q`"
+  assumes I0': "`invar \<and> b \<Rightarrow> p'`"
+  assumes induct_step: "\<lbrace>p'\<rbrace>C \<lbrace>invar\<rbrace>\<^sub>u"  
+  shows "\<lbrace>invar\<rbrace>while\<^sup>\<top> b do C od\<lbrace>q\<rbrace>\<^sub>u"
+  by (rule consequence_hoare_rel[OF uimp_refl _ PHI, 
+                                 OF while_gfp_hoare_rel_minimal_partial[OF uimp_refl],
+                                 OF consequence_hoare_rel[OF I0' induct_step uimp_refl]])    
+
+lemma while_gfp_invr_rel_wp_partial:
+  assumes PHI: "`\<not>b \<and> invar \<Rightarrow> q`"
+  assumes I0': "`invar \<and> b \<Rightarrow> p'`"
+  assumes induct_step: "\<lbrace>p'\<rbrace>C \<lbrace>invar\<rbrace>\<^sub>u"  
+  shows "\<lbrace>invar\<rbrace>invr invar while\<^sup>\<top> b do C od\<lbrace>q\<rbrace>\<^sub>u"                             
+  unfolding while_gfp_invr_rel_def 
+  by (auto intro!: assms while_gfp_rel_consequence_partial)  
+                           
+lemma while_gfp_rel_sp_partial:
+  assumes seq_step: "`p \<Rightarrow> invar`"
+  assumes induct_step: "\<lbrace>invar \<and> b\<rbrace>C \<lbrace>q'\<rbrace>\<^sub>u"
+  assumes I0: "`q' \<Rightarrow> invar`"  
+  shows "\<lbrace>p\<rbrace>while\<^sup>\<top> b do C od\<lbrace>\<not>b \<and> invar\<rbrace>\<^sub>u"
+  by (rule consequence_hoare_rel[OF seq_step _ uimp_refl, 
+                                 OF while_gfp_hoare_rel_minimal_partial[OF uimp_refl],
+                                 OF consequence_hoare_rel[OF uimp_refl induct_step I0]])
+
+lemma while_gfp_invr_rel_sp_partial:
+  assumes seq_step: "`p \<Rightarrow> invar`"
+  assumes induct_step: "\<lbrace>invar \<and> b\<rbrace>C \<lbrace>q'\<rbrace>\<^sub>u"
+  assumes I0: "`q' \<Rightarrow> invar`"  
+  shows "\<lbrace>p\<rbrace>invr invar while\<^sup>\<top> b do C od\<lbrace>\<not>b \<and> invar\<rbrace>\<^sub>u"
+  unfolding while_gfp_invr_rel_def 
+  by (rule consequence_hoare_rel[OF seq_step _ uimp_refl, 
+                                 OF while_gfp_hoare_rel_minimal_partial[OF uimp_refl],
+                                 OF consequence_hoare_rel[OF uimp_refl induct_step I0]])
+                             
+(*TODO:Partial correctness rules for the other rules*)
+                             
+lemma while_lfp_hoare_rel_minimal:
+  assumes WF: "wf R"
+  assumes seq_step: "`p \<Rightarrow> invar`" 
+  assumes induct_step:"\<And>st. \<lbrace>b \<and> invar \<and> e =\<^sub>u \<guillemotleft>st\<guillemotright>\<rbrace>body\<lbrace>invar \<and>(e,\<guillemotleft>st\<guillemotright>)\<^sub>u\<in>\<^sub>u\<guillemotleft>R\<guillemotright>\<rbrace>\<^sub>u"    
+  shows "\<lbrace>p\<rbrace>while\<^sub>\<bottom> b do body od\<lbrace>\<not>b \<and> invar\<rbrace>\<^sub>u"
+  unfolding while_lfp_rel_def_alt
+proof (rule pre_str_hoare_rel[OF seq_step mu_rel_hoare_rel[OF WF if_rel_mono cond_rel_hoare_rel, of _ e]], goal_cases)
+  case (1 st X)
+  assume *: "\<lbrace>invar \<and> (e, \<guillemotleft>st\<guillemotright>)\<^sub>u \<in>\<^sub>u \<guillemotleft>R\<guillemotright>\<rbrace>X\<lbrace>\<not> b \<and> invar\<rbrace>\<^sub>u"  
+  show ?case 
+  proof (rule seq_hoare_rel [of _ _ "invar \<and> (e, \<guillemotleft>st\<guillemotright>)\<^sub>u \<in>\<^sub>u \<guillemotleft>R\<guillemotright>"], goal_cases)
+    case 1
+    then show ?case by (rule induct_step)
+  next
+    case 2
+    then show ?case by (rule *) 
+  qed 
+next
+  case (2 st X)
+  then show ?case by rel_simp 
+qed
+    
+lemma while_lfp_invr_hoare_rel_minimal:
+  assumes WF: "wf R"
+  assumes seq_step: "`p \<Rightarrow> invar`" 
+  assumes induct_step:"\<And>st. \<lbrace>b \<and> invar \<and> e =\<^sub>u \<guillemotleft>st\<guillemotright>\<rbrace>body\<lbrace>invar \<and>(e,\<guillemotleft>st\<guillemotright>)\<^sub>u\<in>\<^sub>u\<guillemotleft>R\<guillemotright>\<rbrace>\<^sub>u"    
+  shows "\<lbrace>p\<rbrace>invr invar while\<^sub>\<bottom> b do body od\<lbrace>\<not>b \<and> invar\<rbrace>\<^sub>u"
+  unfolding while_lfp_invr_rel_def
+  using assms while_lfp_hoare_rel_minimal
+  by blast  
+
+lemma while_lfp_invr_vrt_hoare_rel_minimal:
+  assumes WF: "wf R"
+  assumes seq_step: "`p \<Rightarrow> invar`" 
+  assumes induct_step:"\<And>st. \<lbrace>b \<and> invar \<and> e =\<^sub>u \<guillemotleft>st\<guillemotright>\<rbrace>body\<lbrace>invar \<and>(e,\<guillemotleft>st\<guillemotright>)\<^sub>u\<in>\<^sub>u\<guillemotleft>R\<guillemotright>\<rbrace>\<^sub>u"    
+  shows "\<lbrace>p\<rbrace>invr invar vrt \<guillemotleft>R\<guillemotright> while\<^sub>\<bottom> b do body od\<lbrace>\<not>b \<and> invar\<rbrace>\<^sub>u"
+  unfolding while_lfp_invr_vrt_rel_def
+  using assms while_lfp_hoare_rel_minimal
+  by blast  
+    
+lemma while_lfp_hoare_rel_consequence:
+  assumes WF: "wf R"
+  assumes seq_step: "`p \<Rightarrow> invar`"
+  assumes PHI: "`\<not>b \<and> invar \<Rightarrow> q`"  
+  assumes I0': "\<And>st. `b \<and> invar \<and> e =\<^sub>u \<guillemotleft>st\<guillemotright> \<Rightarrow> p' st`"
+  assumes induct_step: "\<And>st. \<lbrace>p' st\<rbrace>body\<lbrace>q' st\<rbrace>\<^sub>u"
+  assumes  I0: "\<And> st. `q' st \<Rightarrow> invar \<and>(e,\<guillemotleft>st\<guillemotright>)\<^sub>u\<in>\<^sub>u\<guillemotleft>R\<guillemotright> `"
+  shows "\<lbrace>p\<rbrace>while\<^sub>\<bottom> b do body od\<lbrace>q\<rbrace>\<^sub>u" 
+  by (rule consequence_hoare_rel[OF seq_step _ PHI, 
+                                  OF while_lfp_hoare_rel_minimal[OF WF uimp_refl, of _ _ e],
+                                  OF consequence_hoare_rel[OF I0' induct_step I0]])
+
+lemma while_lfp_invr_hoare_rel_consequence:
+  assumes WF: "wf R"
+  assumes seq_step: "`p \<Rightarrow> invar`"
+  assumes PHI: "`\<not>b \<and> invar \<Rightarrow> q`"  
+  assumes I0': "\<And>st. `b \<and> invar \<and> e =\<^sub>u \<guillemotleft>st\<guillemotright> \<Rightarrow> p' st`"
+  assumes induct_step: "\<And>st. \<lbrace>p' st\<rbrace>body\<lbrace>q' st\<rbrace>\<^sub>u"
+  assumes  I0: "\<And> st. `q' st \<Rightarrow> invar \<and>(e,\<guillemotleft>st\<guillemotright>)\<^sub>u\<in>\<^sub>u\<guillemotleft>R\<guillemotright> `"
+  shows "\<lbrace>p\<rbrace>invr invar while\<^sub>\<bottom> b do body od\<lbrace>q\<rbrace>\<^sub>u" 
+  unfolding while_lfp_invr_rel_def
+  by (rule consequence_hoare_rel[OF seq_step _ PHI, 
+                                  OF while_lfp_hoare_rel_minimal[OF WF uimp_refl, of _ _ e],
+                                  OF consequence_hoare_rel[OF I0' induct_step I0]])
+
+lemma while_lfp_invr_vrt_hoare_rel_consequence:
+  assumes WF: "wf R"
+  assumes seq_step: "`p \<Rightarrow> invar`"
+  assumes PHI: "`\<not>b \<and> invar \<Rightarrow> q`"  
+  assumes I0': "\<And>st. `b \<and> invar \<and> e =\<^sub>u \<guillemotleft>st\<guillemotright> \<Rightarrow> p' st`"
+  assumes induct_step: "\<And>st. \<lbrace>p' st\<rbrace>body\<lbrace>q' st\<rbrace>\<^sub>u"
+  assumes  I0: "\<And> st. `q' st \<Rightarrow> invar \<and>(e,\<guillemotleft>st\<guillemotright>)\<^sub>u\<in>\<^sub>u\<guillemotleft>R\<guillemotright> `"
+  shows "\<lbrace>p\<rbrace>invr invar vrt \<guillemotleft>R\<guillemotright> while\<^sub>\<bottom> b do body od\<lbrace>q\<rbrace>\<^sub>u" 
+  unfolding while_lfp_invr_vrt_rel_def  
+  by (rule consequence_hoare_rel[OF seq_step _ PHI, 
+                                 OF while_lfp_hoare_rel_minimal[OF WF uimp_refl, of _ _ e],
+                                 OF consequence_hoare_rel[OF I0' induct_step I0]])
+                              
+lemma while_lfp_hoare_rel_wp:
+  assumes WF: "wf R"
+  assumes PHI: "`\<not>b \<and> invar \<Rightarrow> q`"  
+  assumes I0': "\<And>st. `b \<and> invar \<and> e =\<^sub>u \<guillemotleft>st\<guillemotright> \<Rightarrow> p' st`"
+  assumes induct_step: "\<And>st. \<lbrace>p' st\<rbrace>body\<lbrace>invar \<and>(e,\<guillemotleft>st\<guillemotright>)\<^sub>u\<in>\<^sub>u\<guillemotleft>R\<guillemotright> \<rbrace>\<^sub>u"
+  shows "\<lbrace>invar\<rbrace>while\<^sub>\<bottom> b do body od\<lbrace>q\<rbrace>\<^sub>u" 
+  by (rule consequence_hoare_rel[OF uimp_refl _ PHI,
+                                 OF while_lfp_hoare_rel_minimal[OF WF uimp_refl, of _ _ e],
+                                 OF consequence_hoare_rel[OF I0' induct_step uimp_refl]])
+
+lemma while_lfp_invr_hoare_rel_wp:
+  assumes WF: "wf R"
+  assumes PHI: "`\<not>b \<and> invar \<Rightarrow> q`"  
+  assumes I0': "\<And>st. `b \<and> invar \<and> e =\<^sub>u \<guillemotleft>st\<guillemotright> \<Rightarrow> p' st`"
+  assumes induct_step: "\<And>st. \<lbrace>p' st\<rbrace>body\<lbrace>invar \<and>(e,\<guillemotleft>st\<guillemotright>)\<^sub>u\<in>\<^sub>u\<guillemotleft>R\<guillemotright> \<rbrace>\<^sub>u"
+  shows "\<lbrace>invar\<rbrace>invr invar while\<^sub>\<bottom> b do body od\<lbrace>q\<rbrace>\<^sub>u"                              
+  unfolding while_lfp_invr_rel_def
+  by (rule consequence_hoare_rel[OF uimp_refl _ PHI,
+                                 OF while_lfp_hoare_rel_minimal[OF WF uimp_refl, of _ _ e],
+                                 OF consequence_hoare_rel[OF I0' induct_step uimp_refl]])
+
+lemma while_lfp_invr_vrt_hoare_rel_wp:
+  assumes WF: "wf R"
+  assumes PHI: "`\<not>b \<and> invar \<Rightarrow> q`"  
+  assumes I0': "\<And>st. `b \<and> invar \<and> e =\<^sub>u \<guillemotleft>st\<guillemotright> \<Rightarrow> p' st`"
+  assumes induct_step: "\<And>st. \<lbrace>p' st\<rbrace>body\<lbrace>invar \<and>(e,\<guillemotleft>st\<guillemotright>)\<^sub>u\<in>\<^sub>u\<guillemotleft>R\<guillemotright> \<rbrace>\<^sub>u"
+  shows "\<lbrace>invar\<rbrace>invr invar vrt \<guillemotleft>R\<guillemotright> while\<^sub>\<bottom> b do body od\<lbrace>q\<rbrace>\<^sub>u"                              
+  unfolding while_lfp_invr_vrt_rel_def
+  by (rule consequence_hoare_rel[OF uimp_refl _ PHI,
+                                 OF while_lfp_hoare_rel_minimal[OF WF uimp_refl, of _ _ e],
+                                 OF consequence_hoare_rel[OF I0' induct_step uimp_refl]])
+                                
+lemma while_lfp_hoare_rel_sp:
+  assumes WF: "wf R"
+  assumes seq_step: "`p \<Rightarrow> invar`"
+  assumes induct_step: "\<And>st. \<lbrace>b \<and> invar \<and> e =\<^sub>u \<guillemotleft>st\<guillemotright>\<rbrace>body\<lbrace>q' st\<rbrace>\<^sub>u"
+  assumes  I0: "\<And> st. `q' st \<Rightarrow> invar \<and>(e,\<guillemotleft>st\<guillemotright>)\<^sub>u\<in>\<^sub>u\<guillemotleft>R\<guillemotright> `"
+  shows "\<lbrace>p\<rbrace>while\<^sub>\<bottom> b do body od\<lbrace>\<not>b \<and> invar\<rbrace>\<^sub>u" 
+  by (rule consequence_hoare_rel [OF seq_step _ uimp_refl, 
+                                  OF while_lfp_hoare_rel_minimal[OF WF uimp_refl, of _ _ e],
+                                  OF consequence_hoare_rel[OF uimp_refl induct_step I0]])                              
+                              
+lemma while_lfp_invr_hoare_rel_sp:
+  assumes WF: "wf R"
+  assumes seq_step: "`p \<Rightarrow> invar`"
+  assumes induct_step: "\<And>st. \<lbrace>b \<and> invar \<and> e =\<^sub>u \<guillemotleft>st\<guillemotright>\<rbrace>body\<lbrace>q' st\<rbrace>\<^sub>u"
+  assumes  I0: "\<And> st. `q' st \<Rightarrow> invar \<and>(e,\<guillemotleft>st\<guillemotright>)\<^sub>u\<in>\<^sub>u\<guillemotleft>R\<guillemotright> `"
+  shows "\<lbrace>p\<rbrace>invr invar while\<^sub>\<bottom> b do body od\<lbrace>\<not>b \<and> invar\<rbrace>\<^sub>u" 
+  unfolding while_lfp_invr_rel_def  
+  by (rule consequence_hoare_rel[OF seq_step _ uimp_refl, 
+                                 OF while_lfp_hoare_rel_minimal[OF WF uimp_refl, of _ _ e],
+                                 OF consequence_hoare_rel[OF uimp_refl induct_step I0]])
+
+lemma while_lfp_invr_vrt_hoare_rel_sp:
+  assumes WF: "wf R"
+  assumes seq_step: "`p \<Rightarrow> invar`"
+  assumes induct_step: "\<And>st. \<lbrace>b \<and> invar \<and> e =\<^sub>u \<guillemotleft>st\<guillemotright>\<rbrace>body\<lbrace>q' st\<rbrace>\<^sub>u"
+  assumes  I0: "\<And> st. `q' st \<Rightarrow> invar \<and>(e,\<guillemotleft>st\<guillemotright>)\<^sub>u\<in>\<^sub>u\<guillemotleft>R\<guillemotright> `"
+  shows "\<lbrace>p\<rbrace>invr invar vrt \<guillemotleft>R\<guillemotright> while\<^sub>\<bottom> b do body od\<lbrace>\<not>b \<and> invar\<rbrace>\<^sub>u" 
+  unfolding while_lfp_invr_vrt_rel_def  
+  by (rule consequence_hoare_rel[OF seq_step _ uimp_refl, 
+                                  OF while_lfp_hoare_rel_minimal[OF WF uimp_refl, of _ _ e],
+                                  OF consequence_hoare_rel[OF uimp_refl induct_step I0]])
+  
+subsection {*Hoare for from_until_loop*}     
+
+lemma from_until_lfp_hoare_rel_minimal:
+  assumes WF: "wf R"
+  assumes seq_step: "\<lbrace>p\<rbrace>init\<lbrace>invar\<rbrace>\<^sub>u"
+  assumes induct_step: "\<And>st. \<lbrace>\<not> exit \<and> invar \<and> e =\<^sub>u \<guillemotleft>st\<guillemotright>\<rbrace>body\<lbrace>invar \<and>(e,\<guillemotleft>st\<guillemotright>)\<^sub>u\<in>\<^sub>u\<guillemotleft>R\<guillemotright>\<rbrace>\<^sub>u"
+  shows "\<lbrace>p\<rbrace>from\<^sub>\<bottom> init until exit do body od\<lbrace>exit \<and> invar\<rbrace>\<^sub>u"
+  unfolding from_until_lfp_rel_alt_def while_lfp_rel_def_alt
+  by (rule seq_hoare_rel[OF seq_step, 
+                          OF mu_rel_hoare_rel[OF WF if_rel_mono cond_rel_hoare_rel, of _ e],
+                          OF seq_hoare_rel[OF induct_step], OF _ skip_rel_hoare_rel_intro],                             
+      rel_auto+)
+
+lemma from_until_lfp_invr_hoare_rel_minimal:
+  assumes WF: "wf R"
+  assumes seq_step: "\<lbrace>p\<rbrace>init\<lbrace>invar\<rbrace>\<^sub>u"
+  assumes induct_step: "\<And>st. \<lbrace>\<not> exit \<and> invar \<and> e =\<^sub>u \<guillemotleft>st\<guillemotright>\<rbrace>body\<lbrace>invar \<and>(e,\<guillemotleft>st\<guillemotright>)\<^sub>u\<in>\<^sub>u\<guillemotleft>R\<guillemotright>\<rbrace>\<^sub>u"
+  shows "\<lbrace>p\<rbrace>from\<^sub>\<bottom> init invr invar until exit do body od\<lbrace>exit \<and> invar\<rbrace>\<^sub>u"
+  unfolding from_until_lfp_invr_rel_def 
+  using     from_until_lfp_hoare_rel_minimal [OF WF seq_step induct_step] .
+    
+lemma from_until_lfp_invr_vrt_hoare_rel_minimal:
+  assumes WF: "wf R"
+  assumes seq_step: "\<lbrace>p\<rbrace>init\<lbrace>invar\<rbrace>\<^sub>u"
+  assumes induct_step: "\<And>st. \<lbrace>\<not> exit \<and> invar \<and> e =\<^sub>u \<guillemotleft>st\<guillemotright>\<rbrace>body\<lbrace>invar \<and>(e,\<guillemotleft>st\<guillemotright>)\<^sub>u\<in>\<^sub>u\<guillemotleft>R\<guillemotright>\<rbrace>\<^sub>u"
+  shows "\<lbrace>p\<rbrace>from\<^sub>\<bottom> init invr invar vrt \<guillemotleft>R\<guillemotright> until exit do body od\<lbrace>exit \<and> invar\<rbrace>\<^sub>u"
+  unfolding from_until_lfp_invr_vrt_rel_def 
+  using     from_until_lfp_hoare_rel_minimal [OF WF seq_step induct_step] .
+
+lemma from_until_lfp_hoare_rel_consequence:
+  assumes WF: "wf R"
+  assumes seq_step: "\<lbrace>p\<rbrace>init\<lbrace>invar\<rbrace>\<^sub>u"
+  assumes PHI: "`exit \<and> invar \<Rightarrow> q`"  
+  assumes I0': "\<And>st. `\<not> exit \<and> invar \<and> e =\<^sub>u \<guillemotleft>st\<guillemotright> \<Rightarrow> p' st`"  
+  assumes induct_step: "\<And>st. \<lbrace>p' st\<rbrace>body\<lbrace>q' st\<rbrace>\<^sub>u" 
+  assumes I0: "\<And>st. `q' st \<Rightarrow> invar \<and>(e,\<guillemotleft>st\<guillemotright>)\<^sub>u\<in>\<^sub>u\<guillemotleft>R\<guillemotright>`"     
+  shows "\<lbrace>p\<rbrace>from\<^sub>\<bottom> init until exit do body od\<lbrace>q\<rbrace>\<^sub>u" 
+  unfolding from_until_lfp_rel_alt_def
+  by (simp add: PHI seq_hoare_rel[OF seq_step] 
+                while_lfp_hoare_rel_consequence[OF WF uimp_refl _ I0' induct_step I0])
+
+lemma from_until_lfp_invr_hoare_rel_consequence:
+  assumes WF: "wf R"
+  assumes seq_step: "\<lbrace>p\<rbrace>init\<lbrace>invar\<rbrace>\<^sub>u"
+  assumes PHI: "`exit \<and> invar \<Rightarrow> q`"  
+  assumes I0': "\<And>st. `\<not> exit \<and> invar \<and> e =\<^sub>u \<guillemotleft>st\<guillemotright> \<Rightarrow> p' st`"  
+  assumes induct_step: "\<And>st. \<lbrace>p' st\<rbrace>body\<lbrace>q' st\<rbrace>\<^sub>u" 
+  assumes I0: "\<And>st. `q' st \<Rightarrow> invar \<and>(e,\<guillemotleft>st\<guillemotright>)\<^sub>u\<in>\<^sub>u\<guillemotleft>R\<guillemotright>`"     
+  shows "\<lbrace>p\<rbrace>from\<^sub>\<bottom> init invr invar until exit do body od\<lbrace>q\<rbrace>\<^sub>u"
+  unfolding from_until_lfp_invr_rel_def 
+  using     from_until_lfp_hoare_rel_consequence [OF WF seq_step PHI I0' induct_step I0].
+    
+lemma from_until_lfp_invr_vrt_hoare_rel_consequence:
+  assumes WF: "wf R"
+  assumes seq_step: "\<lbrace>p\<rbrace>init\<lbrace>invar\<rbrace>\<^sub>u"
+  assumes PHI: "`exit \<and> invar \<Rightarrow> q`"  
+  assumes I0': "\<And>st. `\<not> exit \<and> invar \<and> e =\<^sub>u \<guillemotleft>st\<guillemotright> \<Rightarrow> p' st`"  
+  assumes induct_step: "\<And>st. \<lbrace>p' st\<rbrace>body\<lbrace>q' st\<rbrace>\<^sub>u" 
+  assumes I0: "\<And>st. `q' st \<Rightarrow> invar \<and>(e,\<guillemotleft>st\<guillemotright>)\<^sub>u\<in>\<^sub>u\<guillemotleft>R\<guillemotright>`"     
+  shows "\<lbrace>p\<rbrace>from\<^sub>\<bottom> init invr invar vrt \<guillemotleft>R\<guillemotright> until exit do body od\<lbrace>q\<rbrace>\<^sub>u"
+  unfolding from_until_lfp_invr_vrt_rel_def
+  using     from_until_lfp_hoare_rel_consequence [OF WF seq_step PHI I0' induct_step I0].
+ 
+lemma from_until_lfp_hoare_rel_wp:
+  assumes WF: "wf R" 
+  assumes seq_step: "\<lbrace>p\<rbrace>init\<lbrace>invar\<rbrace>\<^sub>u"
+  assumes PHI: "`exit \<and> invar \<Rightarrow> q`"  
+  assumes I0': "\<And>st. `\<not> exit \<and> invar \<and> e =\<^sub>u \<guillemotleft>st\<guillemotright> \<Rightarrow> p' st`"  
+  assumes induct_step: "\<And>st. \<lbrace>p' st\<rbrace>body\<lbrace>invar \<and>(e,\<guillemotleft>st\<guillemotright>)\<^sub>u\<in>\<^sub>u\<guillemotleft>R\<guillemotright>\<rbrace>\<^sub>u" 
+  shows "\<lbrace>p\<rbrace>from\<^sub>\<bottom> init until exit do body od\<lbrace>q\<rbrace>\<^sub>u" 
+  unfolding from_until_lfp_rel_alt_def
+  by (simp add: PHI seq_hoare_rel[OF seq_step]
+                while_lfp_hoare_rel_consequence[OF WF uimp_refl _ I0' induct_step uimp_refl])
+
+lemma from_until_lfp_invr_hoare_rel_wp:
+  assumes WF: "wf R" 
+  assumes seq_step: "\<lbrace>p\<rbrace>init\<lbrace>invar\<rbrace>\<^sub>u"
+  assumes PHI: "`exit \<and> invar \<Rightarrow> q`"  
+  assumes I0': "\<And>st. `\<not> exit \<and> invar \<and> e =\<^sub>u \<guillemotleft>st\<guillemotright> \<Rightarrow> p' st`"  
+  assumes induct_step: "\<And>st. \<lbrace>p' st\<rbrace>body\<lbrace>invar \<and>(e,\<guillemotleft>st\<guillemotright>)\<^sub>u\<in>\<^sub>u\<guillemotleft>R\<guillemotright>\<rbrace>\<^sub>u" 
+  shows "\<lbrace>p\<rbrace>from\<^sub>\<bottom> init invr invar until exit do body od\<lbrace>q\<rbrace>\<^sub>u"
+  unfolding from_until_lfp_invr_rel_def
+  using from_until_lfp_hoare_rel_wp [OF WF seq_step PHI I0' induct_step] .
+    
+lemma from_until_lfp_invr_vrt_hoare_rel_wp:
+  assumes WF: "wf R"   
+  assumes seq_step: "\<lbrace>p\<rbrace>init\<lbrace>invar\<rbrace>\<^sub>u"
+  assumes PHI: "`exit \<and> invar \<Rightarrow> q`"  
+  assumes I0': "\<And>st. `\<not> exit \<and> invar \<and> e =\<^sub>u \<guillemotleft>st\<guillemotright> \<Rightarrow> p' st`"  
+  assumes induct_step: "\<And>st. \<lbrace>p' st\<rbrace>body\<lbrace>invar \<and>(e,\<guillemotleft>st\<guillemotright>)\<^sub>u\<in>\<^sub>u\<guillemotleft>R\<guillemotright>\<rbrace>\<^sub>u" 
+  shows "\<lbrace>p\<rbrace>from\<^sub>\<bottom> init invr invar vrt \<guillemotleft>R\<guillemotright> until exit do body od\<lbrace>q\<rbrace>\<^sub>u"
+  unfolding from_until_lfp_invr_vrt_rel_def
+  using from_until_lfp_hoare_rel_wp[OF WF seq_step PHI I0' induct_step] .
+    
+lemma from_until_lfp_hoare_rel_sp:
+  assumes WF: "wf R"
+  assumes seq_step: "\<lbrace>p\<rbrace>init\<lbrace>q''\<rbrace>\<^sub>u"
+  assumes I0': "`q'' \<Rightarrow> invar`"    
+  assumes induct_step: "\<And>st. \<lbrace>\<not> exit \<and> invar \<and> e =\<^sub>u \<guillemotleft>st\<guillemotright>\<rbrace>body\<lbrace>q' st\<rbrace>\<^sub>u" 
+  assumes I0: "\<And>st. `q' st \<Rightarrow> invar \<and>(e,\<guillemotleft>st\<guillemotright>)\<^sub>u\<in>\<^sub>u\<guillemotleft>R\<guillemotright>`"     
+  shows "\<lbrace>p\<rbrace>from\<^sub>\<bottom> init until exit do body od\<lbrace>exit \<and> invar\<rbrace>\<^sub>u" 
+  unfolding from_until_lfp_rel_alt_def
+  by (simp add: uimp_refl seq_hoare_rel[OF seq_step] pre_str_hoare_rel[OF I0']
+                while_lfp_hoare_rel_consequence[OF WF uimp_refl _ uimp_refl induct_step I0])
+
+lemma from_until_lfp_invr_hoare_rel_sp:
+  assumes WF: "wf R"
+  assumes seq_step: "\<lbrace>p\<rbrace>init\<lbrace>q''\<rbrace>\<^sub>u"
+  assumes I0': "`q'' \<Rightarrow> invar`"  
+  assumes induct_step: "\<And>st. \<lbrace>\<not> exit \<and> invar \<and> e =\<^sub>u \<guillemotleft>st\<guillemotright>\<rbrace>body\<lbrace>q' st\<rbrace>\<^sub>u" 
+  assumes I0: "\<And>st. `q' st \<Rightarrow> invar \<and>(e,\<guillemotleft>st\<guillemotright>)\<^sub>u\<in>\<^sub>u\<guillemotleft>R\<guillemotright>`"     
+  shows "\<lbrace>p\<rbrace>from\<^sub>\<bottom> init invr invar until exit do body od\<lbrace>exit \<and> invar\<rbrace>\<^sub>u" 
+  unfolding from_until_lfp_invr_rel_def
+  using from_until_lfp_hoare_rel_sp[OF WF seq_step I0' induct_step I0] .  
+
+lemma from_until_lfp_invr_vrt_hoare_rel_sp:
+  assumes WF: "wf R"
+  assumes seq_step: "\<lbrace>p\<rbrace>init\<lbrace>q''\<rbrace>\<^sub>u"
+   assumes I0': "`q'' \<Rightarrow> invar`"    
+  assumes induct_step: "\<And>st. \<lbrace>\<not> exit \<and> invar \<and> e =\<^sub>u \<guillemotleft>st\<guillemotright>\<rbrace>body\<lbrace>q' st\<rbrace>\<^sub>u" 
+  assumes I0: "\<And>st. `q' st \<Rightarrow> invar \<and>(e,\<guillemotleft>st\<guillemotright>)\<^sub>u\<in>\<^sub>u\<guillemotleft>R\<guillemotright>`"     
+  shows "\<lbrace>p\<rbrace>from\<^sub>\<bottom> init invr invar vrt \<guillemotleft>R\<guillemotright> until exit do body od\<lbrace>exit \<and> invar\<rbrace>\<^sub>u" 
+  unfolding from_until_lfp_invr_vrt_rel_def
+  using from_until_lfp_hoare_rel_sp[OF WF seq_step I0' induct_step I0] .
+
+subsection {*Hoare for do_while_loop*}     
+
+lemma do_while_lfp_hoare_rel_minimal:
+  assumes WF: "wf R"
+  assumes seq_step: "\<lbrace>p\<rbrace>body\<lbrace>invar\<rbrace>\<^sub>u"  
+  assumes induct_step: "\<And> st. \<lbrace>b \<and> invar \<and>  e =\<^sub>u \<guillemotleft>st\<guillemotright>\<rbrace>body\<lbrace>invar \<and> (e, \<guillemotleft>st\<guillemotright>)\<^sub>u \<in>\<^sub>u \<guillemotleft>R\<guillemotright>\<rbrace>\<^sub>u"
+  shows" \<lbrace>p\<rbrace>do body while\<^sub>\<bottom> b od\<lbrace>\<not>b \<and> invar\<rbrace>\<^sub>u"  
+  unfolding do_while_lfp_rel_alt_def
+  by (rule seq_hoare_rel[OF seq_step while_lfp_hoare_rel_minimal[OF WF uimp_refl induct_step]])  
+
+lemma do_while_lfp_invr_hoare_rel_minimal:
+  assumes WF: "wf R"
+  assumes seq_step: "\<lbrace>p\<rbrace>body\<lbrace>invar\<rbrace>\<^sub>u"  
+  assumes induct_step: "\<And> st. \<lbrace>b \<and> invar \<and>  e =\<^sub>u \<guillemotleft>st\<guillemotright>\<rbrace>body\<lbrace>invar \<and> (e, \<guillemotleft>st\<guillemotright>)\<^sub>u \<in>\<^sub>u \<guillemotleft>R\<guillemotright>\<rbrace>\<^sub>u"
+  shows" \<lbrace>p\<rbrace>do body while\<^sub>\<bottom> b invr invar od\<lbrace>\<not>b \<and> invar\<rbrace>\<^sub>u"  
+  unfolding do_while_lfp_invr_rel_def
+  by (auto intro!: induct_step from_until_lfp_hoare_rel_minimal[OF WF seq_step ])
+ 
+lemma do_while_lfp_invr_vrt_hoare_rel_minimal:
+  assumes WF: "wf R"
+  assumes seq_step: "\<lbrace>p\<rbrace>body\<lbrace>invar\<rbrace>\<^sub>u"  
+  assumes induct_step: "\<And> st. \<lbrace>b \<and> invar \<and>  e =\<^sub>u \<guillemotleft>st\<guillemotright>\<rbrace>body\<lbrace>invar \<and> (e, \<guillemotleft>st\<guillemotright>)\<^sub>u \<in>\<^sub>u \<guillemotleft>R\<guillemotright>\<rbrace>\<^sub>u"
+  shows" \<lbrace>p\<rbrace>do body while\<^sub>\<bottom> b invr invar vrt \<guillemotleft>R\<guillemotright> od\<lbrace>\<not>b \<and> invar\<rbrace>\<^sub>u"  
+  unfolding do_while_lfp_invr_vrt_rel_def
+  by (auto intro!: induct_step from_until_lfp_hoare_rel_minimal[OF WF seq_step ])
+    
+lemma do_while_lfp_hoare_rel_consequence:
+  assumes WF: "wf R"
+  assumes seq_step: "\<lbrace>p\<rbrace>body\<lbrace>invar\<rbrace>\<^sub>u"
+  assumes PHI : "`\<not>b  \<and> invar \<Rightarrow> q`"
+  assumes I0': "\<And>st. `b \<and> invar \<and> e =\<^sub>u \<guillemotleft>st\<guillemotright> \<Rightarrow> p' st`"  
+  assumes induct_step: "\<And> st. \<lbrace>p' st\<rbrace>body\<lbrace>q' st\<rbrace>\<^sub>u"
+  assumes I0: "\<And>st. `q' st \<Rightarrow> invar \<and> (e, \<guillemotleft>st\<guillemotright>)\<^sub>u \<in>\<^sub>u \<guillemotleft>R\<guillemotright>`"  
+  shows "\<lbrace>p\<rbrace>do body while\<^sub>\<bottom> b od\<lbrace>q\<rbrace>\<^sub>u" 
+  unfolding do_while_lfp_rel_alt_def
+  by (rule seq_hoare_rel[OF seq_step 
+                            while_lfp_hoare_rel_consequence[OF WF uimp_refl PHI I0' induct_step I0]])
+    
+lemma do_while_lfp_invr_hoare_rel_consequence:
+  assumes WF: "wf R"
+  assumes seq_step: "\<lbrace>p\<rbrace>body\<lbrace>invar\<rbrace>\<^sub>u"
+  assumes PHI : "`\<not>b  \<and> invar \<Rightarrow> q`"
+  assumes I0': "\<And>st. `b \<and> invar \<and> e =\<^sub>u \<guillemotleft>st\<guillemotright> \<Rightarrow> p' st`"  
+  assumes induct_step: "\<And> st. \<lbrace>p' st\<rbrace>body\<lbrace>q' st\<rbrace>\<^sub>u"
+  assumes I0: "\<And>st. `q' st \<Rightarrow> invar \<and> (e, \<guillemotleft>st\<guillemotright>)\<^sub>u \<in>\<^sub>u \<guillemotleft>R\<guillemotright>`"  
+  shows "\<lbrace>p\<rbrace>do body while\<^sub>\<bottom> b invr invar  od\<lbrace>q\<rbrace>\<^sub>u"
+  unfolding do_while_lfp_invr_rel_def
+  by (auto intro!: assms from_until_lfp_hoare_rel_consequence[OF WF seq_step])
+
+lemma do_while_lfp_invr_vrt_hoare_rel_consequence:
+  assumes WF: "wf R"
+  assumes seq_step: "\<lbrace>p\<rbrace>body\<lbrace>invar\<rbrace>\<^sub>u"
+  assumes PHI : "`\<not>b  \<and> invar \<Rightarrow> q`"
+  assumes I0': "\<And>st. `b \<and> invar \<and> e =\<^sub>u \<guillemotleft>st\<guillemotright> \<Rightarrow> p' st`"  
+  assumes induct_step: "\<And> st. \<lbrace>p' st\<rbrace>body\<lbrace>q' st\<rbrace>\<^sub>u"
+  assumes I0: "\<And>st. `q' st \<Rightarrow> invar \<and> (e, \<guillemotleft>st\<guillemotright>)\<^sub>u \<in>\<^sub>u \<guillemotleft>R\<guillemotright>`"  
+  shows "\<lbrace>p\<rbrace>do body while\<^sub>\<bottom> b invr invar vrt \<guillemotleft>R\<guillemotright> od\<lbrace>q\<rbrace>\<^sub>u"
+  unfolding do_while_lfp_invr_vrt_rel_def
+  by (auto intro!: assms from_until_lfp_hoare_rel_consequence[OF WF seq_step])
+    
+lemma do_while_lfp_hoare_rel_wp:
+  assumes WF: "wf R" 
+  assumes seq_step: "\<lbrace>invar\<rbrace>body\<lbrace>invar\<rbrace>\<^sub>u"
+  assumes PHI : "`\<not>b  \<and> invar \<Rightarrow> q`"
+  assumes I0': "\<And>st. `b \<and> invar \<and> e =\<^sub>u \<guillemotleft>st\<guillemotright> \<Rightarrow> p' st`"  
+  assumes induct_step: "\<And> st. \<lbrace>p' st\<rbrace>body\<lbrace>invar \<and> (e, \<guillemotleft>st\<guillemotright>)\<^sub>u \<in>\<^sub>u \<guillemotleft>R\<guillemotright>\<rbrace>\<^sub>u"
+  shows "\<lbrace>invar\<rbrace>do body while\<^sub>\<bottom> b od\<lbrace>q\<rbrace>\<^sub>u"
+  unfolding do_while_lfp_rel_alt_def
+  by (simp add: uimp_refl seq_hoare_rel[OF seq_step] 
+                while_lfp_hoare_rel_wp[OF WF PHI I0' induct_step])
+
+lemma do_while_lfp_invr_hoare_rel_wp:
+  assumes WF: "wf R"  
+  assumes seq_step: "\<lbrace>invar\<rbrace>body\<lbrace>invar\<rbrace>\<^sub>u"
+  assumes PHI : "`\<not>b \<and> invar \<Rightarrow> q`"
+  assumes I0': "\<And>st. `b \<and> invar \<and> e =\<^sub>u \<guillemotleft>st\<guillemotright> \<Rightarrow> p' st`"  
+  assumes induct_step: "\<And> st. \<lbrace>p' st\<rbrace>body\<lbrace>invar \<and> (e, \<guillemotleft>st\<guillemotright>)\<^sub>u \<in>\<^sub>u \<guillemotleft>R\<guillemotright>\<rbrace>\<^sub>u"
+  shows "\<lbrace>invar\<rbrace>do body while\<^sub>\<bottom> b invr invar od\<lbrace>q\<rbrace>\<^sub>u"
+  unfolding do_while_lfp_invr_rel_def do_while_lfp_rel_alt_def  
+  by (auto intro!: assms from_until_lfp_hoare_rel_wp)
+
+lemma do_while_lfp_invr_vrt_hoare_rel_wp:
+  assumes WF: "wf R"    
+  assumes seq_step: "\<lbrace>invar\<rbrace>body\<lbrace>invar\<rbrace>\<^sub>u"
+  assumes PHI : "`\<not>b \<and> invar \<Rightarrow> q`"
+  assumes I0': "\<And>st. `b \<and> invar \<and> e =\<^sub>u \<guillemotleft>st\<guillemotright> \<Rightarrow> p' st`"  
+  assumes induct_step: "\<And> st. \<lbrace>p' st\<rbrace>body\<lbrace>invar \<and> (e, \<guillemotleft>st\<guillemotright>)\<^sub>u \<in>\<^sub>u \<guillemotleft>R\<guillemotright>\<rbrace>\<^sub>u"
+  shows "\<lbrace>invar\<rbrace>do body while\<^sub>\<bottom> b invr invar vrt \<guillemotleft>R\<guillemotright> od\<lbrace>q\<rbrace>\<^sub>u"
+  unfolding do_while_lfp_invr_vrt_rel_def do_while_lfp_invr_rel_def do_while_lfp_rel_alt_def
+  by (auto intro!: assms from_until_lfp_hoare_rel_wp)
+
+lemma do_while_lfp_hoare_rel_sp:
+  assumes WF: "wf R"
+  assumes seq_step: "\<lbrace>p\<rbrace>body\<lbrace>q''\<rbrace>\<^sub>u"
+  assumes I0': "`q'' \<Rightarrow> invar`"  
+  assumes induct_step: "\<And> st. \<lbrace>b \<and> invar \<and> e =\<^sub>u \<guillemotleft>st\<guillemotright>\<rbrace>body\<lbrace>q' st\<rbrace>\<^sub>u"
+  assumes I0: "\<And>st. `q' st \<Rightarrow> invar \<and> (e, \<guillemotleft>st\<guillemotright>)\<^sub>u \<in>\<^sub>u \<guillemotleft>R\<guillemotright>`"  
+  shows "\<lbrace>p\<rbrace>do body while\<^sub>\<bottom> b od\<lbrace>\<not>b  \<and> invar\<rbrace>\<^sub>u"
+  unfolding  do_while_lfp_rel_alt_def
+  by (simp add: uimp_refl seq_hoare_rel[OF seq_step] pre_str_hoare_rel[OF I0']
+                while_lfp_hoare_rel_sp[OF WF uimp_refl induct_step I0])
+                 
+lemma do_while_lfp_invr_hoare_rel_sp:
+  assumes WF: "wf R"
+  assumes seq_step: "\<lbrace>p\<rbrace>body\<lbrace>q''\<rbrace>\<^sub>u"
+  assumes I0': "`q'' \<Rightarrow> invar`"  
+  assumes induct_step: "\<And> st. \<lbrace>b \<and> invar \<and> e =\<^sub>u \<guillemotleft>st\<guillemotright>\<rbrace>body\<lbrace>q' st\<rbrace>\<^sub>u"
+  assumes I0: "\<And>st. `q' st \<Rightarrow> invar \<and> (e, \<guillemotleft>st\<guillemotright>)\<^sub>u \<in>\<^sub>u \<guillemotleft>R\<guillemotright>`"  
+  shows "\<lbrace>p\<rbrace>do body  while\<^sub>\<bottom> b invr invar od \<lbrace>\<not>b  \<and> invar\<rbrace>\<^sub>u"
+  unfolding do_while_lfp_invr_vrt_rel_def do_while_lfp_invr_rel_def do_while_lfp_rel_alt_def
+  by (auto intro!: assms from_until_lfp_hoare_rel_sp)
+                 
+lemma do_while_lfp_invr_vrt_hoare_rel_sp:
+  assumes WF: "wf R"
+  assumes seq_step: "\<lbrace>p\<rbrace>body\<lbrace>q''\<rbrace>\<^sub>u"
+  assumes I0': "`q'' \<Rightarrow> invar`"  
+  assumes induct_step: "\<And> st. \<lbrace>b \<and> invar \<and> e =\<^sub>u \<guillemotleft>st\<guillemotright>\<rbrace>body\<lbrace>q' st\<rbrace>\<^sub>u"
+  assumes I0: "\<And>st. `q' st \<Rightarrow> invar \<and> (e, \<guillemotleft>st\<guillemotright>)\<^sub>u \<in>\<^sub>u \<guillemotleft>R\<guillemotright>`"  
+  shows "\<lbrace>p\<rbrace>do body while\<^sub>\<bottom> b invr invar vrt \<guillemotleft>R\<guillemotright> od\<lbrace>\<not>b  \<and> invar\<rbrace>\<^sub>u"
+  unfolding do_while_lfp_invr_vrt_rel_def do_while_lfp_rel_alt_def
+  by (auto intro!: assms from_until_lfp_hoare_rel_sp)
+           
+subsection {*Hoare for for_loop*}     
+    
+lemma for_hoare_lfp_rel_minimal:
+  assumes WF: "wf R"
+  assumes seq_step: "\<lbrace>p\<rbrace>init\<lbrace>invar\<rbrace>\<^sub>u"
+  assumes induct_step: "\<And>st. \<lbrace>b \<and> invar \<and> e =\<^sub>u \<guillemotleft>st\<guillemotright>\<rbrace>body ;; incr\<lbrace>invar \<and> (e,\<guillemotleft>st\<guillemotright>)\<^sub>u \<in>\<^sub>u \<guillemotleft>R\<guillemotright>\<rbrace>\<^sub>u" 
+  shows "\<lbrace>p\<rbrace>for\<^sub>\<bottom> (init, b, incr) do body od\<lbrace>\<not>b \<and> invar\<rbrace>\<^sub>u"
+  unfolding for_lfp_rel_def
+  by (auto intro!: assms from_until_lfp_hoare_rel_minimal)
+
+lemma for_lfp_invr_hoare_rel_minimal:
+  assumes WF: "wf R"
+  assumes seq_step: "\<lbrace>p\<rbrace>init\<lbrace>invar\<rbrace>\<^sub>u"
+  assumes induct_step: "\<And>st. \<lbrace>b \<and> invar \<and> e =\<^sub>u \<guillemotleft>st\<guillemotright>\<rbrace>body ;; incr\<lbrace>invar \<and> (e,\<guillemotleft>st\<guillemotright>)\<^sub>u \<in>\<^sub>u \<guillemotleft>R\<guillemotright>\<rbrace>\<^sub>u" 
+  shows "\<lbrace>p\<rbrace>for\<^sub>\<bottom> (init, b, incr) invr invar do body od\<lbrace>\<not>b \<and> invar\<rbrace>\<^sub>u"
+  unfolding for_lfp_invr_rel_def for_lfp_rel_def
+  by (simp add: from_until_lfp_hoare_rel_minimal [OF WF seq_step, of _ e] induct_step)  
+
+lemma for_lfp_invr_vrt_hoare_rel_minimal:
+  assumes WF: "wf R"
+  assumes seq_step: "\<lbrace>p\<rbrace>init\<lbrace>invar\<rbrace>\<^sub>u"
+  assumes induct_step: "\<And>st. \<lbrace>b \<and> invar \<and> e =\<^sub>u \<guillemotleft>st\<guillemotright>\<rbrace>body ;; incr\<lbrace>invar \<and> (e,\<guillemotleft>st\<guillemotright>)\<^sub>u \<in>\<^sub>u \<guillemotleft>R\<guillemotright>\<rbrace>\<^sub>u" 
+  shows "\<lbrace>p\<rbrace>for\<^sub>\<bottom> (init, b, incr) invr invar vrt \<guillemotleft>R\<guillemotright> do body od\<lbrace>\<not>b \<and> invar\<rbrace>\<^sub>u"
+  unfolding for_lfp_invr_vrt_rel_def for_lfp_rel_def
+  by (simp add: from_until_lfp_hoare_rel_minimal [OF WF seq_step, of _ e] induct_step)      
+
+lemma for_lfp_hoare_rel_consequence:
+  assumes WF: "wf R"
+  assumes seq_step:  "\<lbrace>p\<rbrace>init\<lbrace>invar\<rbrace>\<^sub>u"
+  assumes PHI: "`\<not>b \<and> invar \<Rightarrow>q`"  
+  assumes I0': "\<And>st. `b \<and> invar \<and> e =\<^sub>u \<guillemotleft>st\<guillemotright> \<Rightarrow> p' st`"  
+  assumes induct_step: "\<And>st. \<lbrace>p' st\<rbrace>body;;incr\<lbrace>q' st\<rbrace>\<^sub>u"
+  assumes I0: "\<And>st. `q' st \<Rightarrow> invar \<and> (e, \<guillemotleft>st\<guillemotright>)\<^sub>u \<in>\<^sub>u \<guillemotleft>R\<guillemotright>`"
+  shows "\<lbrace>p\<rbrace>for\<^sub>\<bottom> (init, b, incr) do body od\<lbrace>q\<rbrace>\<^sub>u"  
+  unfolding for_lfp_rel_def
+  by(simp add: from_until_lfp_hoare_rel_consequence [OF WF seq_step PHI _ induct_step I0] I0')
+
+lemma for_lfp_invr_hoare_rel_consequence:
+  assumes WF: "wf R"
+  assumes seq_step:  "\<lbrace>p\<rbrace>init\<lbrace>invar\<rbrace>\<^sub>u"
+  assumes PHI: "`\<not>b \<and> invar \<Rightarrow>q`"  
+  assumes I0': "\<And>st. `b \<and> invar \<and> e =\<^sub>u \<guillemotleft>st\<guillemotright> \<Rightarrow> p' st`"  
+  assumes induct_step: "\<And>st. \<lbrace>p' st\<rbrace>body;;incr\<lbrace>q' st\<rbrace>\<^sub>u"
+  assumes I0: "\<And>st. `q' st \<Rightarrow> invar \<and> (e, \<guillemotleft>st\<guillemotright>)\<^sub>u \<in>\<^sub>u \<guillemotleft>R\<guillemotright>`"
+  shows "\<lbrace>p\<rbrace>for\<^sub>\<bottom> (init, b, incr) invr invar do body od\<lbrace>q\<rbrace>\<^sub>u"  
+  unfolding for_lfp_rel_def for_lfp_invr_rel_def
+  by(simp add: from_until_lfp_hoare_rel_consequence [OF WF seq_step PHI _ induct_step I0] I0')
+
+lemma for_lfp_invr_vrt_hoare_rel_consequence:
+  assumes WF: "wf R"
+  assumes seq_step:  "\<lbrace>p\<rbrace>init\<lbrace>invar\<rbrace>\<^sub>u"
+  assumes PHI: "`\<not>b \<and> invar \<Rightarrow>q`"  
+  assumes I0': "\<And>st. `b \<and> invar \<and> e =\<^sub>u \<guillemotleft>st\<guillemotright> \<Rightarrow> p' st`"  
+  assumes induct_step: "\<And>st. \<lbrace>p' st\<rbrace>body;;incr\<lbrace>q' st\<rbrace>\<^sub>u"
+  assumes I0: "\<And>st. `q' st \<Rightarrow> invar \<and> (e, \<guillemotleft>st\<guillemotright>)\<^sub>u \<in>\<^sub>u \<guillemotleft>R\<guillemotright>`"
+  shows "\<lbrace>p\<rbrace>for\<^sub>\<bottom> (init, b, incr) invr invar vrt \<guillemotleft>R\<guillemotright> do body od\<lbrace>q\<rbrace>\<^sub>u"  
+  unfolding for_lfp_rel_def for_lfp_invr_vrt_rel_def
+  by(simp add: from_until_lfp_hoare_rel_consequence [OF WF seq_step PHI _ induct_step I0] I0')
+    
+lemma for_lfp_hoare_rel_wp:
+  assumes WF : "wf R"  
+  assumes seq_step: "\<lbrace>p\<rbrace>init\<lbrace>invar\<rbrace>\<^sub>u"
+  assumes PHI: "`\<not>b \<and> invar \<Rightarrow>q`"  
+  assumes I0': "\<And>st. `b \<and> invar \<and> e=\<^sub>u \<guillemotleft>st\<guillemotright> \<Rightarrow> p' st`"
+  assumes induct_step: "\<And>st. \<lbrace>p' st\<rbrace>body;;incr\<lbrace>invar \<and> (e, \<guillemotleft>st\<guillemotright>)\<^sub>u \<in>\<^sub>u \<guillemotleft>R\<guillemotright>\<rbrace>\<^sub>u"
+  shows "\<lbrace>p\<rbrace>for\<^sub>\<bottom> (init,b,incr) do body od\<lbrace>q\<rbrace>\<^sub>u"
+  unfolding for_lfp_rel_alt_def
+  by (simp add: uimp_refl seq_hoare_rel[OF seq_step] 
+                while_lfp_hoare_rel_wp[OF WF PHI I0' induct_step])
+
+lemma for_lfp_invr_hoare_rel_wp:
+  assumes WF : "wf R"  
+  assumes seq_step: "\<lbrace>p\<rbrace>init\<lbrace>invar\<rbrace>\<^sub>u"
+  assumes PHI: "`\<not>b \<and> invar \<Rightarrow>q`"  
+  assumes I0': "\<And>st. `b \<and> invar \<and> e=\<^sub>u \<guillemotleft>st\<guillemotright> \<Rightarrow> p' st`"
+  assumes induct_step: "\<And>st. \<lbrace>p' st\<rbrace>body;;incr\<lbrace>invar \<and> (e, \<guillemotleft>st\<guillemotright>)\<^sub>u \<in>\<^sub>u \<guillemotleft>R\<guillemotright>\<rbrace>\<^sub>u"
+  shows "\<lbrace>p\<rbrace>for\<^sub>\<bottom> (init,b,incr) invr invar do body od\<lbrace>q\<rbrace>\<^sub>u"
+  unfolding for_lfp_invr_rel_def for_lfp_rel_alt_def from_until_lfp_rel_alt_def
+  by (simp add: seq_hoare_rel[OF seq_step] 
+                while_lfp_hoare_rel_wp[OF WF PHI I0' induct_step])
+
+lemma for_lfp_invr_vrt_hoare_rel_wp:
+  assumes WF : "wf R"
+  assumes seq_step: "\<lbrace>p\<rbrace>init\<lbrace>invar\<rbrace>\<^sub>u"
+  assumes PHI: "`\<not>b \<and> invar \<Rightarrow>q`"  
+  assumes I0': "\<And>st. `b \<and> invar \<and> e=\<^sub>u \<guillemotleft>st\<guillemotright> \<Rightarrow> p' st`"
+  assumes induct_step: "\<And>st. \<lbrace>p' st\<rbrace>body;;incr\<lbrace>invar \<and> (e, \<guillemotleft>st\<guillemotright>)\<^sub>u \<in>\<^sub>u \<guillemotleft>R\<guillemotright>\<rbrace>\<^sub>u"
+  shows "\<lbrace>p\<rbrace>for\<^sub>\<bottom> (init,b,incr) invr invar vrt \<guillemotleft>R\<guillemotright> do body od\<lbrace>q\<rbrace>\<^sub>u"
+  unfolding for_lfp_invr_vrt_rel_def for_lfp_rel_alt_def from_until_lfp_rel_alt_def
+  by (simp add: uimp_refl seq_hoare_rel[OF seq_step] 
+                while_lfp_hoare_rel_wp[OF WF  PHI I0' induct_step])
+
+lemma for_lfp_hoare_rel_sp:
+  assumes WF: "wf R"
+  assumes seq_step:"\<lbrace>p\<rbrace>init\<lbrace>q''\<rbrace>\<^sub>u"
+  assumes I0': "`q'' \<Rightarrow> invar`"  
+  assumes induct_step: "\<And>st. \<lbrace>b \<and> invar \<and> e =\<^sub>u \<guillemotleft>st\<guillemotright>\<rbrace>body;;incr\<lbrace>q' st\<rbrace>\<^sub>u"
+  assumes I0: "\<And>st. `q' st \<Rightarrow> invar \<and> (e, \<guillemotleft>st\<guillemotright>)\<^sub>u \<in>\<^sub>u \<guillemotleft>R\<guillemotright>`"  
+  shows "\<lbrace>p\<rbrace>for\<^sub>\<bottom> (init,b,incr) do body od\<lbrace>\<not>b \<and> invar\<rbrace>\<^sub>u"
+  unfolding for_lfp_rel_alt_def  
+  by (simp add: seq_hoare_rel[OF seq_step] pre_str_hoare_rel[OF I0']
+                while_lfp_hoare_rel_sp[OF WF uimp_refl induct_step I0])
+ 
+lemma for_lfp_invr_hoare_rel_sp:
+  assumes WF: "wf R"
+  assumes seq_step:"\<lbrace>p\<rbrace>init\<lbrace>q''\<rbrace>\<^sub>u"
+  assumes I0':  "`q'' \<Rightarrow> invar`"
+  assumes induct_step: "\<And>st. \<lbrace>b \<and> invar \<and> e =\<^sub>u \<guillemotleft>st\<guillemotright>\<rbrace>body;;incr\<lbrace>q' st\<rbrace>\<^sub>u"
+  assumes I0: "\<And>st. `q' st \<Rightarrow> invar \<and> (e, \<guillemotleft>st\<guillemotright>)\<^sub>u \<in>\<^sub>u \<guillemotleft>R\<guillemotright>`"  
+  shows "\<lbrace>p\<rbrace>for\<^sub>\<bottom> (init,b,incr) invr invar do body od\<lbrace>\<not>b \<and> invar\<rbrace>\<^sub>u"
+  unfolding for_lfp_invr_rel_def for_lfp_rel_alt_def from_until_lfp_rel_alt_def
+  by (simp add: seq_hoare_rel[OF seq_step] pre_str_hoare_rel[OF I0']
+                while_lfp_hoare_rel_sp[OF WF uimp_refl induct_step I0])
+         
+lemma for_lfp_invr_vrt_hoare_rel_sp:
+  assumes WF: "wf R"
+  assumes seq_step:"\<lbrace>p\<rbrace>init\<lbrace>q''\<rbrace>\<^sub>u"
+  assumes I0':"`q''\<Rightarrow> invar`" 
+  assumes induct_step: "\<And>st. \<lbrace>b \<and> invar \<and> e =\<^sub>u \<guillemotleft>st\<guillemotright>\<rbrace>body;;incr\<lbrace>q' st\<rbrace>\<^sub>u"
+  assumes I0: "\<And>st. `q' st \<Rightarrow> invar \<and> (e, \<guillemotleft>st\<guillemotright>)\<^sub>u \<in>\<^sub>u \<guillemotleft>R\<guillemotright>`"  
+  shows "\<lbrace>p\<rbrace>for\<^sub>\<bottom> (init,b,incr) invr invar vrt \<guillemotleft>R\<guillemotright> do body od\<lbrace>\<not>b \<and> invar\<rbrace>\<^sub>u"
+  unfolding for_lfp_invr_vrt_rel_def for_lfp_rel_alt_def  from_until_lfp_rel_alt_def
+  by (simp add: seq_hoare_rel[OF seq_step] pre_str_hoare_rel[OF I0']
+                while_lfp_hoare_rel_sp[OF WF uimp_refl induct_step I0])
+      
+lemmas loop_invr_vrt_hoare_rel_sp_instantiated [hoare_sp_rules] = 
+       while_lfp_invr_vrt_hoare_rel_sp [where e = "&\<Sigma>"]
+       for_lfp_invr_vrt_hoare_rel_sp [where e = "&\<Sigma>"]
+       do_while_lfp_invr_vrt_hoare_rel_sp [where e = "&\<Sigma>"]
+       from_until_lfp_invr_vrt_hoare_rel_sp[where e = "&\<Sigma>"]
+
+lemmas loop_invr_vrt_hoare_rel_wp_instantiated [hoare_wp_rules] = 
+       while_lfp_invr_vrt_hoare_rel_wp [where e = "&\<Sigma>"]
+       for_lfp_invr_vrt_hoare_rel_wp [where e = "&\<Sigma>"]
+       do_while_lfp_invr_vrt_hoare_rel_wp [where e = "&\<Sigma>"]
+       from_until_lfp_invr_vrt_hoare_rel_wp[where e = "&\<Sigma>"]
 
 end
 
